

# Fundamentals of Artificial Intelligence

## Laboratory

Dr. Mauro Dragoni

Department of Information Engineering and Computer Science  
Academic Year 2022/2023

## Exercise 9.1

- Consider the following axioms:
  1. If something is intelligent, it has common sense
  2. Deep Blue does not have common sense
  3. (Conclusion) Deep Blue is not intelligent

## Exercise 9.1

- Resolution
  1. If something is intelligent, it has common sense  
 $\forall x (I(x) \Rightarrow H(x))$
  2. Deep Blue does not have common sense  
 $\neg H(D)$
  3. (Conclusion) Deep Blue is not intelligent  
 $\neg I(D)$

## Exercise 9.1

- Resolution

1. If something is intelligent, it has common sense

$$\forall x (I(x) \Rightarrow H(x))$$

$$\neg I(x) \vee H(x)$$

2. Deep Blue does not have common sense

$$\neg H(D)$$

3. (Conclusion) Deep Blue is not intelligent

$$\neg I(D)$$

$$I(D) \text{ (negated conclusion)}$$

## Exercise 9.1

- Resolution

1. If something is intelligent, it has common sense

$$\forall x (I(x) \Rightarrow H(x))$$

$$\neg I(x) \vee H(x)$$

2. Deep Blue does not have common sense

$$\neg H(D)$$

3. (Conclusion) Deep Blue is not intelligent

$$\neg I(D)$$

$$I(D) \text{ (negated conclusion)}$$

4. [1, 2]  $\neg I(D)$      $\{x/D\}$

## Exercise 9.1

- Resolution

1. If something is intelligent, it has common sense

$$\forall x I(x) \Rightarrow H(x)$$

$$\neg I(x) \vee H(x)$$

2. Deep Blue does not have common sense

$$\neg H(D)$$

3. (Conclusion) Deep Blue is not intelligent

$$\neg I(D)$$

$$I(D) \text{ (negated conclusion)}$$

4. [1, 2]  $\neg I(D)$      $\{x/D\}$

5. [3, 4]  $\square$

## Exercise 9.2

- Consider the following axioms:
  1.  $\text{Mother}(\text{Lulu}, \text{Fifi})$
  2.  $\text{Alive}(\text{Lulu})$
  3.  $\forall x \forall y (\text{Mother}(x,y) \Rightarrow \text{Parent}(x,y))$
  4.  $\forall x \forall y ((\text{Parent}(x,y) \wedge \text{Alive}(x)) \Rightarrow \text{Older}(x,y))$
  5. (Conclusion)  $\text{Older}(\text{Lulu}, \text{Fifi})$

## Exercise 9.2

- Consider the following axioms:
  1. **Mother(Lulu, Fifi)**
  2. **Alive(Lulu)**
  3.  $\forall x \forall y (\text{Mother}(x,y) \Rightarrow \text{Parent}(x,y))$   
 **$\neg \text{Mother}(x,y) \vee \text{Parent}(x,y)$**
  4.  $\forall x \forall y ((\text{Parent}(x,y) \wedge \text{Alive}(x)) \Rightarrow \text{Older}(x,y))$   
 **$\neg \text{Parent}(x,y) \vee \neg \text{Alive}(x) \vee \text{Older}(x,y)$**
  5. (Conclusion) **Older(Lulu, Fifi)**  
 **$\neg \text{Older}(\text{Lulu}, \text{Fifi})$**



## Exercise 9.2

- Consider the following axioms:

1. **Mother(Lulu, Fifi)**

2. **Alive(Lulu)**

3.  $\forall x \forall y (\text{Mother}(x,y) \Rightarrow \text{Parent}(x,y))$   
 **$\neg \text{Mother}(x,y) \vee \text{Parent}(x,y)$**

4.  $\forall x \forall y ((\text{Parent}(x,y) \wedge \text{Alive}(x)) \Rightarrow \text{Older}(x,y))$   
 **$\neg \text{Parent}(x,y) \vee \neg \text{Alive}(x) \vee \text{Older}(x,y)$**

5. (Conclusion) **Older(Lulu, Fifi)**  
 **$\neg \text{Older}(\text{Lulu}, \text{Fifi})$**

6. [1, 3]    **Parent(Lulu,Fifi)**                      {x/Lulu, y/Fifi}

## Exercise 9.2

- Consider the following axioms:

1. **Mother(Lulu, Fifi)**

2. **Alive(Lulu)**

3.  $\forall x \forall y (\text{Mother}(x,y) \Rightarrow \text{Parent}(x,y))$   
 **$\neg \text{Mother}(x,y) \vee \text{Parent}(x,y)$**

4.  $\forall x \forall y ((\text{Parent}(x,y) \wedge \text{Alive}(x)) \Rightarrow \text{Older}(x,y))$   
 **$\neg \text{Parent}(x,y) \vee \neg \text{Alive}(x) \vee \text{Older}(x,y)$**

5. (Conclusion) **Older(Lulu, Fifi)**  
 **$\neg \text{Older}(\text{Lulu}, \text{Fifi})$**

6. [1, 3] **Parent(Lulu, Fifi)**  $\{x/\text{Lulu}, y/\text{Fifi}\}$

7. [4, 6]  **$\neg \text{Alive}(\text{Lulu}) \vee \text{Older}(\text{Lulu}, \text{Fifi})$**   $\{x/\text{Lulu}, y/\text{Fifi}\}$

## Exercise 9.2

- Consider the following axioms:

1. **Mother(Lulu, Fifi)**

2. **Alive(Lulu)**

3.  $\forall x \forall y (\text{Mother}(x,y) \Rightarrow \text{Parent}(x,y))$   
 **$\neg \text{Mother}(x,y) \vee \text{Parent}(x,y)$**

4.  $\forall x \forall y ((\text{Parent}(x,y) \wedge \text{Alive}(x)) \Rightarrow \text{Older}(x,y))$   
 **$\neg \text{Parent}(x,y) \vee \neg \text{Alive}(x) \vee \text{Older}(x,y)$**

5. (Conclusion) **Older(Lulu, Fifi)**  
 **$\neg \text{Older}(\text{Lulu}, \text{Fifi})$**

6. [1, 3] **Parent(Lulu, Fifi)**  $\{x/\text{Lulu}, y/\text{Fifi}\}$

7. [4, 6]  **$\neg \text{Alive}(\text{Lulu}) \vee \text{Older}(\text{Lulu}, \text{Fifi})$**   $\{x/\text{Lulu}, y/\text{Fifi}\}$

8. [2, 7] **Older(Lulu, Fifi)**

## Exercise 9.2

- Consider the following axioms:

1. **Mother(Lulu, Fifi)**

2. **Alive(Lulu)**

3.  $\forall x \forall y (\text{Mother}(x,y) \Rightarrow \text{Parent}(x,y))$   
 **$\neg \text{Mother}(x,y) \vee \text{Parent}(x,y)$**

4.  $\forall x \forall y ((\text{Parent}(x,y) \wedge \text{Alive}(x)) \Rightarrow \text{Older}(x,y))$   
 **$\neg \text{Parent}(x,y) \vee \neg \text{Alive}(x) \vee \text{Older}(x,y)$**

5. (Conclusion) **Older(Lulu, Fifi)**  
 **$\neg \text{Older}(\text{Lulu}, \text{Fifi})$**

6. [1, 3] **Parent(Lulu, Fifi)**  $\{x/\text{Lulu}, y/\text{Fifi}\}$

7. [4, 6]  **$\neg \text{Alive}(\text{Lulu}) \vee \text{Older}(\text{Lulu}, \text{Fifi})$**   $\{x/\text{Lulu}, y/\text{Fifi}\}$

8. [2, 7] **Older(Lulu, Fifi)**

9. [5, 8]  $\square$

## Exercise 9.3

- Axioms:

1.  $\text{Allergies}(x) \Rightarrow \text{Sneeze}(x)$
2.  $\text{Cat}(y) \wedge \text{AllergicToCats}(x) \Rightarrow \text{Allergies}(x)$
3.  $\text{Cat}(\text{Felix})$
4.  $\text{AllergicToCats}(\text{Mary})$
5. (Conclusion)  $\text{Sneeze}(\text{Mary})$

## Exercise 9.3

- Axioms:

1.  $\text{Allergies}(x) \Rightarrow \text{Sneeze}(x)$   
 $\neg \text{Allergies}(w) \vee \text{Sneeze}(w)$
2.  $\text{Cat}(y) \wedge \text{AllergicToCats}(x) \Rightarrow \text{Allergies}(x)$   
 $\neg \text{Cat}(y) \vee \neg \text{AllergicToCats}(z) \vee \text{Allergies}(z)$
3.  $\text{Cat}(\text{Felix})$
4.  $\text{AllergicToCats}(\text{Mary})$
5. (Conclusion)  $\text{Sneeze}(\text{Mary})$   
 $\neg \text{Sneeze}(\text{Mary})$

## Exercise 9.3

- Axioms:

1.  $\neg \text{Allergies}(w) \vee \text{Sneeze}(w)$
2.  $\neg \text{Cat}(y) \vee \neg \text{AllergicToCats}(z) \vee \text{Allergies}(z)$
3.  $\text{Cat}(\text{Felix})$
4.  $\text{AllergicToCats}(\text{Mary})$
5. (Conclusion)  $\neg \text{Sneeze}(\text{Mary})$
6.  $[1, 2] \quad \neg \text{Cat}(y) \vee \text{Sneeze}(z) \vee \neg \text{AllergicToCats}(z) \quad \{w/z\}$

## Exercise 9.3

- Axioms:

1.  $\neg \text{Allergies}(w) \vee \text{Sneeze}(w)$
2.  $\neg \text{Cat}(y) \vee \neg \text{AllergicToCats}(z) \vee \text{Allergies}(z)$
3.  $\text{Cat}(\text{Felix})$
4.  $\text{AllergicToCats}(\text{Mary})$
5. (Conclusion)  $\neg \text{Sneeze}(\text{Mary})$
6. [1, 2]  $\neg \text{Cat}(y) \vee \text{Sneeze}(z) \vee \neg \text{AllergicToCats}(z)$   $\{w/z\}$
7. [3, 6]  $\text{Sneeze}(z) \vee \neg \text{AllergicToCats}(z)$   $\{y/\text{Felix}\}$



## Exercise 9.3

- Axioms:

1.  $\neg \text{Allergies}(w) \vee \text{Sneeze}(w)$
2.  $\neg \text{Cat}(y) \vee \neg \text{AllergicToCats}(z) \vee \text{Allergies}(z)$
3.  $\text{Cat}(\text{Felix})$
4.  $\text{AllergicToCats}(\text{Mary})$
5. (Conclusion)  $\neg \text{Sneeze}(\text{Mary})$
6. [1, 2]  $\neg \text{Cat}(y) \vee \text{Sneeze}(z) \vee \neg \text{AllergicToCats}(z)$   $\{w/z\}$
7. [3, 6]  $\text{Sneeze}(z) \vee \neg \text{AllergicToCats}(z)$   $\{y/\text{Felix}\}$
8. [4, 7]  $\text{Sneeze}(\text{Mary})$   $\{z/\text{Mary}\}$

## Exercise 9.3

- Axioms:

1.  $\neg \text{Allergies}(w) \vee \text{Sneeze}(w)$
2.  $\neg \text{Cat}(y) \vee \neg \text{AllergicToCats}(z) \vee \text{Allergies}(z)$
3.  $\text{Cat}(\text{Felix})$
4.  $\text{AllergicToCats}(\text{Mary})$
5. (Conclusion)  $\neg \text{Sneeze}(\text{Mary})$
6. [1, 2]  $\neg \text{Cat}(y) \vee \text{Sneeze}(z) \vee \neg \text{AllergicToCats}(z)$   $\{w/z\}$
7. [3, 6]  $\text{Sneeze}(z) \vee \neg \text{AllergicToCats}(z)$   $\{y/\text{Felix}\}$
8. [4, 7]  $\text{Sneeze}(\text{Mary})$   $\{z/\text{Mary}\}$
9. [5, 8]  $\square$

## Exercise 9.6

Consider the following set of clauses, build a refutation using the Hyper-Resolution strategy:

- (1)  $Q(c) \vee R(b) \vee T(e)$
- (2)  $\neg Q(c) \vee T(e) \vee \neg S(d)$
- (3)  $Q(c) \vee S(d)$
- (4)  $S(d) \vee T(e)$
- (5)  $\neg T(e) \vee R(b)$
- (6)  $\neg R(b) \vee \neg P(a)$
- (7)  $R(b) \vee P(a)$
- (8)  $P(a)$

## Exercise 9.6

Consider the following set of clauses, build a refutation using the Hyper-Resolution strategy:

$$(1) \quad Q(c) \vee R(b) \vee T(e)$$

$$(2) \quad \neg Q(c) \vee T(e) \vee \neg S(d)$$

$$(3) \quad Q(c) \vee S(d)$$

$$(4) \quad S(d) \vee T(e)$$

$$(5) \quad \neg T(e) \vee R(b)$$

$$(6) \quad \neg R(b) \vee \neg P(a)$$

$$(7) \quad R(b) \vee P(a)$$

$$(8) \quad P(a)$$

$$(9) \quad [1,2] \quad R(b) \vee T(e) \vee \neg S(d)$$

$$(10) \quad [9,4] \quad R(b) \vee T(e)$$

$$(11) \quad [10,5] \quad R(b)$$

$$(12) \quad [6,8] \quad \neg R(b)$$

$$(13) \quad [11,12] \quad \{\}$$

## Exercise 9.7

Consider the following set of clauses, build a refutation using the Hyper-Resolution strategy:

- (1)  $P(a) \vee Q(c) \vee R(b)$
- (2)  $\neg U(a) \vee R(b)$
- (3)  $\neg P(a) \vee R(b) \vee T(e)$
- (4)  $\neg Q(c) \vee T(e) \vee \neg S(d)$
- (5)  $\neg R(b) \vee U(a)$
- (6)  $S(d) \vee T(e)$
- (7)  $\neg T(e) \vee R(b)$
- (8)  $\neg R(b)$

## Exercise 9.7

Consider the following set of clauses, build a refutation using the Hyper-Resolution strategy:

(1)  $P(a) \vee Q(c) \vee R(b)$

(2)  $\neg U(a) \vee R(b)$

(3)  $\neg P(a) \vee R(b) \vee T(e)$

(4)  $\neg Q(c) \vee T(e) \vee \neg S(d)$

(5)  $\neg R(b) \vee U(a)$

(6)  $S(d) \vee T(e)$

(7)  $\neg T(e) \vee R(b)$

(8)  $\neg R(b)$

(9) [1,3]  $Q(c) \vee R(b) \vee T(e)$

(10) [9,4]  $R(b) \vee T(e) \vee \neg S(d)$

(11) [10,6]  $R(b) \vee T(e)$

(12) [11,7]  $R(b)$

(13) [8,12]  $\{\}$

## Exercise 9.8

Consider the following set of clauses, build a refutation using the Hyper-Resolution strategy:

- (1)  $Q(c) \vee S(b) \vee T(e)$
- (2)  $\neg Q(c) \vee T(e) \vee \neg U(d)$
- (3)  $Q(c) \vee U(d)$
- (4)  $U(d) \vee T(e)$
- (5)  $\neg T(e) \vee S(b)$
- (6)  $\neg S(b) \vee \neg R(a)$
- (7)  $S(b) \vee R(a)$
- (8)  $R(a)$

## Exercise 9.8

Consider the following set of clauses, build a refutation using the Hyper-Resolution strategy:

$$(1) \quad Q(c) \vee S(b) \vee T(e)$$

$$(2) \quad \neg Q(c) \vee T(e) \vee \neg U(d)$$

$$(3) \quad Q(c) \vee U(d)$$

$$(4) \quad U(d) \vee T(e)$$

$$(5) \quad \neg T(e) \vee S(b)$$

$$(6) \quad \neg S(b) \vee \neg R(a)$$

$$(7) \quad S(b) \vee R(a)$$

$$(8) \quad R(a)$$

$$(9) \quad [1,2] \quad S(b) \vee T(e) \vee \neg U(d)$$

$$(10) \quad [9,4] \quad S(b) \vee T(e)$$

$$(11) \quad [10,5] \quad S(b)$$

$$(12) \quad [6,8] \quad \neg S(b)$$

$$(13) \quad [11,12] \quad \{\}$$



## Exercise 9.4

- Consider the following axioms:  
(predicates to use: HOUND, HOWL, HAVE, CAT, MOUSE, LS)
  1. All hounds howl at night.
  2. Anyone who has any cats will not have any mice.
  3. Light sleepers do not have anything which howls at night.
  4. John has either a cat or a hound.
  5. (Conclusion) If John is a light sleeper, then John does not have any mice.

## Exercise 9.4

- The conclusion can be proved using Resolution as shown in the next slides.
  - The first step is to write each axiom as a well-formed formula in first-order predicate calculus. The clauses written for the above axioms are shown below, using LS(x) for “light sleeper”.
1. All hounds howl at night.  
 $\forall x (\text{HOUND}(x) \Rightarrow \text{HOWL}(x))$
  2. Anyone who has any cats will not have any mice.  
 $\forall x \forall y (\text{HAVE}(x,y) \wedge \text{CAT}(y) \Rightarrow \neg \exists z (\text{HAVE}(x,z) \wedge \text{MOUSE}(z)))$
  3. Light sleepers do not have anything which howls at night.  
 $\forall x (\text{LS}(x) \Rightarrow \neg \exists y (\text{HAVE}(x,y) \wedge \text{HOWL}(y)))$
  4. John has either a cat or a hound.  
 $\exists x (\text{HAVE}(\text{John},x) \wedge (\text{CAT}(x) \vee \text{HOUND}(x)))$
  5. (Conclusion) If John is a light sleeper, then John does not have any mice.  
 $\text{LS}(\text{John}) \Rightarrow \neg \exists z (\text{HAVE}(\text{John},z) \wedge \text{MOUSE}(z))$

## Exercise 9.4

- The next step is to transform each well-formed formula into Prenex Normal Form, skolemize, and rewrite as clauses in conjunctive normal form.

1. All hounds howl at night.

$$\forall x (\text{HOUND}(x) \Rightarrow \text{HOWL}(x))$$

$$\neg \text{HOUND}(x) \vee \text{HOWL}(x)$$

## Exercise 9.4

- The next step is to transform each wff into Prenex Normal Form, skolemize, and rewrite as clauses in conjunctive normal form; these transformations are shown below.

2. Anyone who has any cats will not have any mice.

$$\forall x \forall y (\text{HAVE}(x,y) \wedge \text{CAT}(y) \Rightarrow \neg \exists z (\text{HAVE}(x,z) \wedge \text{MOUSE}(z)))$$

$$\forall x \forall y (\text{HAVE}(x,y) \wedge \text{CAT}(y) \Rightarrow \forall z \neg (\text{HAVE}(x,z) \wedge \text{MOUSE}(z)))$$

$$\forall x \forall y \forall z (\neg (\text{HAVE}(x,y) \wedge \text{CAT}(y)) \vee \neg (\text{HAVE}(x,z) \wedge \text{MOUSE}(z)))$$

$$\neg \text{HAVE}(x,y) \vee \neg \text{CAT}(y) \vee \neg \text{HAVE}(x,z) \vee \neg \text{MOUSE}(z)$$

## Exercise 9.4

- The next step is to transform each wff into Prenex Normal Form, skolemize, and rewrite as clauses in conjunctive normal form; these transformations are shown below.

3. Light sleepers do not have anything which howls at night.

$$\forall x (LS(x) \Rightarrow \neg \exists y (HAVE(x,y) \wedge HOWL(y)))$$

$$\forall x (LS(x) \Rightarrow \forall y \neg (HAVE(x,y) \wedge HOWL(y)))$$

$$\forall x \forall y (LS(x) \Rightarrow \neg HAVE(x,y) \vee \neg HOWL(y))$$

$$\forall x \forall y (\neg LS(x) \vee \neg HAVE(x,y) \vee \neg HOWL(y))$$

$$\neg LS(x) \vee \neg HAVE(x,y) \vee \neg HOWL(y)$$

## Exercise 9.4

- The next step is to transform each wff into Prenex Normal Form, skolemize, and rewrite as clauses in conjunctive normal form; these transformations are shown below.

4. John has either a cat or a hound.

$$\exists x (\text{HAVE}(\text{John}, x) \wedge (\text{CAT}(x) \vee \text{HOUND}(x)))$$
$$\text{HAVE}(\text{John}, a) \wedge (\text{CAT}(a) \vee \text{HOUND}(a))$$

## Exercise 9.4

- The next step is to transform each wff into Prenex Normal Form, skolemize, and rewrite as clauses in conjunctive normal form; these transformations are shown below.

5. (Conclusion) If John is a light sleeper, then John does not have any mice.

$LS(\text{John}) \Rightarrow \neg \exists z (\text{HAVE}(\text{John}, z) \wedge \text{MOUSE}(z))$

$\neg[LS(\text{John}) \Rightarrow \neg \exists z (\text{HAVE}(\text{John}, z) \wedge \text{MOUSE}(z))]$  (negated conclusion)

$\neg[\neg LS(\text{John}) \vee \neg \exists z (\text{HAVE}(\text{John}, z) \wedge \text{MOUSE}(z))]$

$LS(\text{John}) \wedge \exists z (\text{HAVE}(\text{John}, z) \wedge \text{MOUSE}(z))$

**$LS(\text{John}) \wedge \text{HAVE}(\text{John}, b) \wedge \text{MOUSE}(b)$**

## Exercise 9.4

- The set of CNF clauses for this problem is thus as follows:

1.  $\neg \text{HOUND}(x) \vee \text{HOWL}(x)$

2.  $\neg \text{HAVE}(x,y) \vee \neg \text{CAT}(y) \vee \neg \text{HAVE}(x,z) \vee \neg \text{MOUSE}(z)$

3.  $\neg \text{LS}(x) \vee \neg \text{HAVE}(x,y) \vee \neg \text{HOWL}(y)$

4.

a.  $\text{HAVE}(\text{John}, a)$

b.  $\text{CAT}(a) \vee \text{HOUND}(a)$

5.

a.  $\text{LS}(\text{John})$

b.  $\text{HAVE}(\text{John}, b)$

c.  $\text{MOUSE}(b)$